---
layout:      post
title:       "Exercise 3.5: Equivalent Forms of Entropy"
sorting_tag: "0305"
tags:        [chapter 3]
comments:    true
---

The $$\phi$$-entropy is defined by

\begin{equation}
    \Hb_\phi(X) = \E[\phi(X)] - \phi(\E[X]).
\end{equation}

Let $$L$$ be a linear function.
Then

\begin{align}
    \Hb_{\phi + L}(X)
    &= \E[\phi(X)] + \E[L(X)] - \phi(\E[X]) - L(\E[X]) \newline
    &= \E[\phi(X)] - \phi(\E[X]) \newline
    &= \Hb_{\phi}(X).
\end{align}

For example, the entropy defined by $$\phi(u) = u \log u - u$$ gives the same the entropy as defined by $$\phi(u) = u \log u$$.