---
layout:      post
title:       "Exercise 3.16: Different Forms of Functional Bernstein Inequality"
sorting_tag: "316"
tags:        [chapter 3]
comments:    true
---

## (a)

Let $$t = \frac{n \delta^2}{c_1 \gamma^2 + c_2 b \delta}$$. Using the quadratic
formula, we can solve for $$\delta$$
\begin{align}
  \delta
  &=
  \frac{
    c\_2 b t + \sqrt{c\_2^2 b^2 t^2 + 4 c\_1 n \gamma^2 t}
  }{
    2n
  }
  \newline
  &\leq
  \frac{
    2 c\_2 b t + 2 \gamma \sqrt{c\_1 n t}
  }{
    2 n
  }
  =
  \frac{c\_2 b t}{n}
  +
  \gamma
  \sqrt{\frac{c\_1 t}{n}}
  \, ,
\end{align}
where we used $$\sqrt{a^2 + b^2} \leq a + b$$ for $$a, b \geq 0$$.


## (b)

We will w.l.o.g. assume that $$\mathscr{F}$$ is symmetrised, i.e., for every
$$f \in \mathscr{F}$$, $$-f \in \mathscr{F}$$. This ensures that the
random variable
\begin{align}
  Z = \sup\_{f \in \mathscr{F}} \frac{1}{n} \sum\_{i=1}^n f(X\_i)
  \, ,
\end{align}
is almost surely non-negative, and thus $$\E[Z] \geq 0$$.

Substituting the bound for $$\gamma^2 \leq \sigma^2 + c_3 b \E [Z]$$ and using
the $$\sqrt{a^2 + b^2} \leq a + b$$ for $$a, b \geq 0 $$ inequality
\begin{align}
  \gamma
  \sqrt{\frac{c\_1 t}{n}}
  \leq
  \sigma \sqrt{\frac{c\_1 t}{n}}
  +
  \sqrt{\frac{c\_1 c\_3 b t \E [Z]}{n}}
  \, ,
\end{align}
where we are using $$\E[Z] \geq 0$$ from above. Since for any $$\epsilon > 0$$
\begin{align}
  \left(
    \sqrt{\frac{c_1 c_3 b t}{2 \epsilon n}}
    -
    \sqrt{\epsilon \E[Z]}
  \right)^2
  =
  \frac{c\_1 c\_3 bt}{2 \epsilon n}
  +
  \epsilon \E [Z]
  -
  \sqrt{2 \frac{c\_1 c\_3 b t \E [Z]}{n}}
  \geq
  0
  \, ,
\end{align}
we can upper bound
\begin{align}
  \sqrt{\frac{c\_1 c\_3 b t \E [Z]}{n}}
  \leq
  \frac{c\_1 c\_3 b t}{2 \sqrt{2} \varepsilon n}
  +
  \frac{\epsilon \E[Z]}{\sqrt{2}}
  \, .
\end{align}
The required result can be obtained by upper bounding the right hand side by its
$$\sqrt{2}$$ multiple, and substituting the implied bound
\begin{align}
  \gamma
  \sqrt{\frac{c\_1 t}{n}}
  \leq
  \sigma \sqrt{\frac{c\_1 t}{n}}
  +
  \frac{c\_1 c\_3 b t}{2 \varepsilon n}
  +
  \epsilon \E[Z]
  \, ,
\end{align}
into our result from (a).
