---
layout:      post
title:       "Exercise 3.15: Bounds for Suprema of Non-Negative Functions"
sorting_tag: "0315"
tags:        [chapter 3]
comments:    true
---

Let $$(V_i)_{i=1}^n$$ be an i.i.d. sequence of random variables and $$\F$$ a class of functions taking values in $$[0, 1]$$.
Consider

\begin{equation}
    Z = \sup_{f \in \F} \sum_{i=1}^n f(V_i).
\end{equation}

Without loss of generality, assume that $$\F = \set{f^1, \ldots, f^m}.$$
Define

\begin{equation}
    X_i = (f^1(V_i), \ldots, f^m(V_i))
\end{equation}

and consider the function

\begin{equation}
    Z(X) = \max_{j \in [m]} \sum_{i=1}^n X^j_i.
\end{equation}


## (a)

Let $$Y_k(X)$$ be equal to $$X$$ except with the $$k^{\text{th}}$$.
This eliminates one term in the sum of $$Z$$, hence can only decrease it, so

\begin{equation}
    Z(X) \ge Z(Y_k(X))
    \iff
    Z(X) - Z(Y_k(X)) \ge 0.
\end{equation}


## (b)

By tensorisation of the entropy, we have

\begin{equation}
    \Hb(e^{\lambda Z_k(X)})
    \le \E\sbrac{
        \sum_{i=1}^n \Hb(e^{\lambda Z_i(X)} \cond X_{-i})
    }
\end{equation}

where $$Z_i(X)$$ is the function $$X_i \to Z(X)$$ with all other elements fixed.
Therefore, by the variational representation of the entropy,

\begin{equation}
    \Hb(e^{\lambda Z_k(X)})
    \le \E\sbrac{
        \sum_{i=1}^n \E[\psi(\lambda(Z(X) - Z(Y_i(X)))) e^{\lambda Z(X)} \cond X_{-i}]
    }
\end{equation}

where $$\psi(u) = e^{-u} - 1 + u$$.

## (c)

Let $$\Ab_l$$ be the collection of realisations of $$X$$ that achieves the maximum at index $$l$$.
Without loss of generality, assume $$(\Ab_l)_{l=1}^m$$ to be disjoint.
Then, if $$X \in \Ab_l$$,

\begin{equation}
    Z(X) - Z(Y_k(X))
    = \sum_{i=1}^n X^l_i - Z(Y_k(X))
    \le X^l_k
\end{equation}

by lower bounding the maximum of $$Z(Y_k(X))$$ by index $$l$$.
Therefore, multiply by $$\lambda \ge 0$$ and sum against $$\ind(X \in \Ab_l)$$ to find

\begin{equation}
    0
    \le \lambda (Z(X) - Z(Y_k(X)))
    \le \lambda \sum_{l = 1}^m \ind (X \in \Ab_l) X^l_k.
\end{equation}


## (d)

For $$\alpha \le 1$$, observe that that $$\psi(\alpha x) \le \alpha \psi(x)$$.
Hence, using that

\begin{equation}
    \sum_{l = 1}^m \ind (X \in \Ab_l) X^l_k \le 1
\end{equation}

because every function in $$\F$$ takes values in $$[0, 1]$$, we obtain

\begin{equation}
    0
    \le \psi(\lambda(Z(X) - Z(Y_k(X))))
    \le \psi(\lambda) \sum_{l = 1}^m \ind (X \in \Ab_l) X^l_k,
\end{equation}

also using that $$\psi$$ is increasing.

## (e)

Combining the previous parts, we find

\begin{equation}
    \Hb(e^{\lambda Z_k(X)})
    \le \psi(\lambda) \E\sbrac{
        \sum_{l = 1}^m\ind (X \in \Ab_l) \sum_{i=1}^nX^l_i e^{\lambda Z(X)}
    }
    = \psi(\lambda) \E[Z(X) e^{\lambda Z(X)}],
\end{equation}

by definition of $$\Ab_l$$.

## (f)

Part (e) gives that

\begin{equation}
    \lambda \varphi'(\lambda) - \varphi(\lambda) \log \varphi(\lambda)
    \le \psi(\lambda) \varphi'(\lambda).
\end{equation}

Divide by $$\varphi(\lambda) > 0$$:

\begin{equation}
    \lambda (\log \varphi)'(\lambda) - \log \varphi(\lambda)
    \le \psi(\lambda) (\log \varphi)'(\lambda).
\end{equation}

Hence, rearranging,

\begin{equation}
    (\log \varphi)'(\lambda)
    \le \frac{1}{\lambda - \psi(\lambda)} \log \varphi(\lambda)
    = \frac{e^{\lambda}}{e^{\lambda} - 1} \log \varphi(\lambda),
\end{equation}

using that $$\lambda - \psi(\lambda) > 0$$.
Because not $$Z(X) = 0$$ a.s., it holds that $$\log \varphi(\lambda) > 0$$, so this differential inequality can be rewritten as

\begin{equation}
    (\log \log \varphi)'(\lambda) \le (\log(\exp - 1))'(\lambda).
\end{equation}

Therefore,

\begin{equation}
    \parens{\log \frac{\log \varphi}{\exp - 1}}'(\lambda) \le 0,
\end{equation}

and integrating gives, for $$\lambda > \lambda_0 > 0$$,

\begin{equation}
    \log \frac{\log \varphi(\lambda)}{e^{\lambda} - 1}
    \le \log \frac{\log \varphi(\lambda_0)}{e^{\lambda_0} - 1}
    \to \log \varphi'(0)
    = \log \E[Z(X)],
\end{equation}

by taking $$\lambda_0 \downarrow 0$$ and using L'Hopital's rule.
We conclude that

\begin{equation}
    \log \varphi(\lambda) \le (e^{\lambda} - 1) \E[Z(X)]
\end{equation}

for all $$\lambda \ge 0$$.