---
layout:      post
title:       "Exercise 2.15"
sorting_tag: "215"
tags:        [chapter 2, bounded differences inequality]
comments:    true
---

We show that
\begin{equation}
    g(x_1, \ldots, x_n) = \norm{\hat f_n - f}_1
\end{equation}
has bounded differences, where $$\hat f_n$$ is the KDE for observations $$x_1,\ldots,x_n$$.
This follows directly from the reverse triangle inequality:
\begin{align}
    \abs{g(x, x_2,\ldots, x_n) - g(y, x_2, \ldots, x_n)}
    &\le \norm{\hat f_n(x) - \hat f_n(y)}_1 \newline
    &= \frac{1}{nh} \int \abs{
        K\parens{\frac{z - x}{h}}
        - K\parens{\frac{z - y}{h}}
    } \isd z \newline
    &\le \frac{2}{n}\norm{K}_1 = \frac{2}{n}.
\end{align}
Therefore, by the Bounded Differences Inequality,
\begin{equation}
    \P(\norm{\hat f_n - f}_1 - \E[\norm{\hat f_n - f}_1] \ge t)
    \le e^{-\frac12 n t^2}.
\end{equation}