---
layout:      post
title:       "Exercise 3.4: Entropy and Constant Shifts"
sorting_tag: "0304"
tags:        [chapter 3]
comments:    true
---

## (a)

\begin{align}
  \mathbb{H} (e^{\lambda X})
  &=
  e^{\lambda c} \left\lbrace
    \E [\lambda (X + c) e^{\lambda X}]
    -
    \E [e^{\lambda X}]
    \log \E [e^{\lambda (X + c)}]
  \right\rbrace
  \newline
  &=
  e^{\lambda c} \left\lbrace
    \E [\lambda X e^{\lambda X}]
    +
    \lambda c \E [e^{\lambda X}]
    -
    \E [e^{\lambda X}]
    \log \E [e^{\lambda X}]
    -
    \lambda c \E [e^{\lambda X}]
  \right\rbrace
  \newline
  &=
  e^{\lambda c} \mathbb{H} (e^{\lambda X})
  \, .
\end{align}

## (b)

This follows by the MGF identity
$$ \varphi_{X + c} (\lambda) = e^{\lambda c} \varphi_X (\lambda) $$ combined
with (a).
