---
layout:      post
title:       "Exercise 3.10: Brunnâ€“Minkowski and Classical Isoperimetric Inequality"
sorting_tag: "310"
tags:        [chapter 3]
comments:    true
---

This exercise proves that the following versions of the Brunn-Minkowski
inequality are equivalent:
\begin{align}
  \label{eq:bm1}\tag{BM1}
  \vol(A + B)^{1/n}
  &\geq
  \vol(A)^{1/n} + \vol(B)^{1/n}
  \newline
  \label{eq:bm2}
  \tag{BM2}
  \vol(\lambda A + (1 - \lambda) B)^{1 / n}
  &\geq
  \lambda \vol(A)^{1/n}
  +
  (1 - \lambda)
  \vol(B)^{1/n}
  \newline
  \label{eq:bm3}
  \tag{BM3}
  \vol(\lambda A + (1 - \lambda)B)
  &\geq
  \vol(A)^{\lambda}
  \vol(B)^{1 - \lambda}
  \, ,
\end{align}
where $$ \lambda \in [0, 1] $$ and $$ A , B $$ are (closed compact) convex
bodies in $$\R^n$$.

Throughout we will be using the following identity which holds for any $$c \geq 0$$ and $$A \in \R^n$$
\begin{align}
  \vol(c A) = c^n \vol(A)
  \, .
\end{align}


## (a) $$\eqref{eq:bm1} \iff \eqref{eq:bm2}$$

For the $$\eqref{eq:bm1} \implies \eqref{eq:bm2}$$ direction
\begin{align}
  \vol(\lambda A + (1 - \lambda) B)^{1 / n}
  &\geq
  \vol(\lambda A)^{1/n}
  +
  \vol((1 - \lambda) B)^{1/n}
  \newline
  &=
  \lambda \vol(A)^{1/n}
  +
  (1 - \lambda) \vol(B)^{1/n}
  \, .
\end{align}
For the reverse direction
\begin{align}
  \vol(A + B)^{1/n}
  =
  2\vol\left(\tfrac{1}{2} A + \tfrac{1}{2} B\right)^{1/n}
  \geq
  \vol(A)^{1/n}
  +
  \vol(B)^{1/n}
  \, .
\end{align}


## (b) $$\eqref{eq:bm2} \implies \eqref{eq:bm3}$$

By the weighted AM-GM inequality (or Jensen's inequality)
\begin{align}
  \lambda \vol(A)^{1/n}
  +
  (1 - \lambda) \vol(B)^{1/n}
  \geq
  \vol(A)^{\lambda / n}
  \vol(B)^{(1 - \lambda) / n}
  \, .
\end{align}


## (c) $$\eqref{eq:bm3} \implies \eqref{eq:bm2}$$

If either $$\vol(A)$$ or $$\vol(B)$$ equals zero, the claim is trivial.
Otherwise define $$C = \tfrac{A}{\vol(A)^{1/n}}$$,
$$D = \tfrac{B}{\vol(B)^{1/n}}$$, and
\begin{align}
  \delta
  =
  \frac{
    \lambda \vol(A)^{1/n}
  }{
    \lambda \vol(A)^{1/n} + (1 - \lambda) \vol(B)^{1/n}
  }
  \, .
\end{align}
Observing $$\vol(C) = \vol(D) = 1$$, \eqref{eq:bm3} implies
\begin{align}
  \vol\left(
    \delta C + (1 - \delta) D
  \right)^{1 / n}
  =
  \vol \left(
    \frac{
      \lambda A + (1 - \lambda) B
    }{
      \lambda \vol(A)^{1/n} + (1 - \lambda) \vol(B)^{1/n}
    }
  \right)^{1/n}
  \geq
  1
  \, .
\end{align}
