---
layout:      post
title:       "Exercise 3.3: Variational Representation of Entropy"
sorting_tag: "33"
tags:        [chapter 3]
comments:    true
---

Using that $$\psi(u) = e^{-u} - 1 + u$$, expand

\begin{equation}
    \E[\psi(\lambda(X - t)) e^{\lambda X}]
    = e^{\lambda t} - \E[e^{\lambda X}] + \E[\lambda X e^{\lambda X}] - \lambda t \E[e^{\lambda X}].
\end{equation}

Set the derivative to zero:

\begin{equation}
    \lambda e^{\lambda t} - \lambda \E[e^{\lambda X}] = 0
    \implies
    \lambda t = \log \E[e^{\lambda X}].
\end{equation}

Therefore,

\begin{equation}
    \min_{t \in \R}\, \E[\psi(\lambda(X - t)) e^{\lambda X}]
    = \E[\lambda X e^{\lambda X}] - \E[e^{\lambda X}] \log \E[e^{\lambda X}]
    = \Hb(e^{\lambda X}).
\end{equation}
