---
layout:      post
title:       "Exercise 14.5: Empirical Approximations of Kernel Integral Operators"
sorting_tag: "1405"
tags:        [chapter 14]
comments:    true
---

## (a)
We take it that that $\E[\hat T\_k] = T\_k$ means that $\E[\hat T\_k(f)] = T\_k(f)$ for all $f \in \Hb$:
\begin{equation}
    \E[\hat T\_k(f)]
    = \frac1n \sum\_{i=1}^n \E[f(x\_i)k(x\_i, \vardot)]
    = \frac1n \sum\_{i=1}^n T\_k(f)
    = T\_k(f).
\end{equation}

## (b)
Note that $\hat T\_k - T\_k$ is a bounded and self-adjoint operator on $\Hb$.
Therefore, we have the following characterisation:
\begin{equation}
    \norm{\hat T\_k - T\_k}\_\Hb
    = \sup\_{\norm{f}\_\Hb \le 1} |\langle f, (\hat T\_k - T\_k) f\rangle\_\Hb|.
\end{equation}
Note that
\begin{equation}
    |\langle f, (\hat T\_k - T\_k) f\rangle\_\Hb|
    = |\langle f, \hat T\_k f\rangle\_\Hb - \langle f, T\_k f\rangle\_\Hb|
    = |\norm{f}^2\_n - \norm{f}^2\_2|,
\end{equation}
which is immediately amenable to techniques from the chapter.

## (c)
Bound
\begin{equation}
    \norm{\hat T\_k \phi\_j - \mu\_j \phi\_j}\_\Hb
    = \norm{\hat T\_k \phi\_j - T\_k \phi\_j}\_\Hb
    \le \norm{\hat T\_k - T\_k}\_\Hb \norm{\phi\_j}\_\Hb
\end{equation}
and note that
\begin{equation}
    \norm{\phi\_j}\_\Hb
    = \frac{1}{\mu\_j} \norm{T\_k \phi\_j}\_\Hb
\end{equation}
where
\begin{equation}
    \norm{T\_k \phi\_j}\_\Hb^2
    = \E[\phi\_j(X) \phi\_j(Y) k(X, Y)]
    \le \sqrt{\E[\phi\_j^2(X) \phi^2\_j(Y)] \E[k^2(X, Y)]}
    = \norm{k}\_{L^2(\P \otimes \P)}^2.
\end{equation}
Therefore,
\begin{equation}
    \norm{\hat T\_k \phi\_j - \mu\_j \phi\_j}\_\Hb
    \le \frac{\norm{k}\_{L^2(\P \otimes \P)}}{\mu\_j} \norm{\hat T\_k - T\_k}\_\Hb.
\end{equation}