---
layout:      post
title:       "Exercise 4.3: Maximum Likelihood and Uniform Laws"
sorting_tag: "0403"
tags:        [chapter 4, incomplete]
comments:    true
---

## (a)
### (i)
We have
\begin{equation}
    p_\th(x) = \frac{e^{\th x}}{1 + e^{\th}}
\end{equation}
with
\begin{equation}
    \E_\th[X] = \frac{e^{\th}}{1 + e^{\th}}
\end{equation}
Therefore,

\begin{equation}
    \E_{\th^\*}\sbrac{\log \frac{p_{\th^\*}(X)}{p_{\th}(X)}}
    =
        \log \frac{1 + e^{\th}}{1 + e^{\th^\*}}
        + (\th^\* - \th) \frac{e^{\th^\*}}{1 + e^{\th^\*}}.
\end{equation}

### (ii)
We have
\begin{equation}
    p_\th(x) = \frac{1}{x!}e^{\th x} e^{-e^{\th}}
\end{equation}
with
\begin{equation}
    \E_\th[X]
    = e^{-e^{\th}} \sum_{x=0}^\infty \frac{1}{x!}e^{\th x}
    = e^{-e^{\th}} (e^{e^{\th}})'
    = e^{\th}.
\end{equation}
Therefore,
\begin{equation}
    \E_{\th^\*}\sbrac{\log \frac{p_{\th^\*}(X)}{p_{\th}(X)}}
    =
        (\th^\* - \th) e^{\th^\*} - (e^{\th^\*} - e^{\th}).
\end{equation}

### (iii)
This is a standard result:
\begin{equation}
    \KL(p_{\th^\*}, p_{\th})
    = \frac12\parens{
        \tr(\Sigma (\Sigma^\*)^{-1})
        + \log \frac{\det \Sigma}{\det \Sigma^\*}
        + (\mu - \mu^\*)^\T \Sigma^{-1}(\mu - \mu^\*)
        - n
    }.
\end{equation}
