---
layout:      post
title:       "Exercise 13.11: Differentiable Functions and Fourier Coefficients"
sorting_tag: "1311"
tags:        [chapter 13]
comments:    true
---

## (a)
By regularity--decay duality of the Fourier transform and the Fourier--Plancherel theorem,
\begin{equation}
    \norm{\F(\partial^{(\alpha)} f)\_n}\_{\ell^2}^2
    \overset{\text{(dual.)}}{=} \norm{(2 \pi i n)^{(\alpha)} \hat f\_n}\_{\ell^2}^2
    \overset{\text{(F.--P.)}}{=} \norm{\partial^{(\alpha)} f}\_{L^2[0,1]}^2
    \le R.
\end{equation}
Therefore,
\begin{equation}
    \sum\_{n=0}^\infty n^{2 \alpha} (\hat f\_n)^2 \lesssim R.
\end{equation}
Suppose that $(\hat f\_n)^2 \gtrsim R n^{-(2 \alpha + 1)}$.
Then
\begin{equation}
    R \gtrsim \sum\_{n=0}^\infty n^{2 \alpha} (\hat f\_n)^2 \gtrsim R \sum\_{n=0}^\infty \frac1n,
\end{equation}
which would mean that the harmonic series is convergent, a contradiction.
Therefore,
\begin{equation}
    (\hat f\_n)^2 \lesssim R n^{-(2 \alpha + 1)},
\end{equation}
which is stronger than required.

## (b)
From Example 13.14, we have that
\begin{equation}
    \inf\_{f \in \G(1;M)} \norm{f - f^\*}\_{L^2(\P)}^2
    = \sum\_{m=M+1}^\infty (\hat f^\*\_m)^2.
\end{equation}
Therefore, using (a),
\begin{equation}
    \inf\_{f \in \G(1;M)} \norm{f - f^\*}\_{L^2(\P)}^2
    \lesssim R \sum\_{m=M+1}^\infty n^{-(2 \alpha + 1)}
    \le R \int\_{M}^\infty x^{-(2 \alpha + 1)} \isd x
    = \frac{R}{2 \alpha} M^{-2 \alpha}.
\end{equation}