---
layout:      post
title:       "Exercise 12.15: Sobolev Kernels and Norms"
sorting_tag: "1215"
tags:        [chapter 12]
comments:    true
---

Follows directly from Proposition 12.27, which allow us to add the norms of $\Hb_1$ and $\Hb_2$.
The norm of $\Hb_2$ follows from Example 12.17, and we now identify the norm of $\Hb_1$.

For $\Hb_1$, we show that the inner product is given by

\begin{equation} \label{eq:inner-product}
    \lra{f, g}\_{\Hb\_1} = \sum_{\ell=0}^{\alpha - 1} f^{(\ell)}(0) g^{(\ell)}(0)
\end{equation}

by showing that the reproducing property is true for the kernel

\begin{equation}
    k_1(x, z) = \sum_{\ell = 0}^{\alpha - 1} \frac{x^\ell}{\ell!}\frac{z^\ell}{\ell!}.
\end{equation}

Since there is only one Hilbert space for which the reproducing property is true for the kernel $k_1$ (Moore--Aronszajn theorem), \eqref{eq:inner-product} must indeed be the inner product for $\Hb_1$, which means that the norm of $\Hb_1$ is given by

\begin{equation}
    \norm{f}\_{\Hb\_1}
    = \lra{f, f}\_{\Hb\_1}
    = \sum_{\ell=0}^{\alpha - 1} (f^{(\ell)}(0))^2.
\end{equation}

Consider a polynomial of degree $\alpha - 1$:

\begin{equation}
    f(x) = \sum_{\ell=0}^{\alpha - 1} a_i x^\ell.
\end{equation}

Then, by a Taylor expansion of $f$ around $x = 0$,

\begin{equation}
    f(x)
    = \sum_{\ell=0}^{\alpha - 1} \frac{x^{\ell}}{\ell!} f^{(\ell)}(0) 
    \overset{(\*)}{=} \lra{k(x, \vardot), f}\_{\Hb\_1}
\end{equation}

where equality $(\*)$ follows from the observation that

\begin{equation}
    \left.\left(\frac{\sd}{\sd z}\right)^\ell k_1(x, z)\right|\_{z = 0} = \frac{x^{\ell}}{\ell!}.
\end{equation}



